completed part 8

UseHoare.v
@@ -26,7 +26,12 @@ Proof.
   intros A B.
   apply auto_hoare'; simpl.
   unfold update_state; simpl.
-Admitted.
+  intros.
+  destruct H as [HA HB].
+  split.
+  - apply HB.
+  - apply HA. 
+Qed.
 
 Definition slow_assign : stmt :=
   While
@@ -43,7 +48,16 @@ Proof.
   intros.
   apply auto_hoare'; simpl.
   unfold update_state; simpl.
-Admitted.
+  intros.
+  split.
+  - apply H.
+  - intros.
+    split.
+    + intros.
+      lia.
+    + intros.
+      lia. 
+Qed.
 
 Definition dummy_sum (x y: Z) :=
   Seq
@@ -52,7 +66,7 @@ Definition dummy_sum (x y: Z) :=
       (Assign "y" (Const y))
       (While
         (Lt (Const 0) (Var "y"))
-         (fun env => True)
+         (fun env => eval_expr env (Var "y") >= 0 /\ (eval_expr env (Var "x")) + (eval_expr env (Var "y")) = x + y)
         (Seq
           (Assign "x" (Add (Var "x") (Const 1)))
           (Assign "y" (Sub (Var "y") (Const 1)))
@@ -63,19 +77,29 @@ Definition dummy_sum (x y: Z) :=
 Theorem dummy_sum_correct x y:
   0 <= y
   -> valid_hoare_triple
-       (fun _ => True)
+       (fun env => env "y" >= 0 /\ env "x" + env "y" = x + y)
        (dummy_sum x y)
        (fun env => env "x" = x + y).
 Proof.
   intros.
   apply auto_hoare'.
   simpl; unfold update_state; simpl; intros.
-Admitted.
+  split.
+  - lia.
+  - intros.
+    split.
+    + intros.
+      split.
+      * lia.
+      * lia.
+    + intros.
+      lia. 
+Qed.
 
 Definition gcd (x y : Z) :=
   While
     (Not (Eq (Var "x") (Var "y")))
-       (fun env => True)
+       (fun env => Z.gcd (env "x") (env "y") = Z.gcd x y)
     (If
       (Lt (Var "x") (Var "y"))
       (Assign "y" (Sub (Var "y") (Var "x")))
@@ -95,7 +119,37 @@ Theorem gcd_correct:
 Proof.
   intros. apply auto_hoare'.
   simpl. unfold update_state; simpl.
-Admitted.
+  intros.
+  destruct H as [Hx Hy].
+  split.
+  - rewrite Hx.
+    rewrite Hy.
+    reflexivity.
+  - intros.
+    split.
+    + intros.
+      split.
+      * intros.
+        rewrite <- H1.
+        apply Z.gcd_sub_diag_r.
+      * intros.
+        rewrite <- H1.
+        assert (Z.gcd (env' "x" - env' "y") (env' "y") = Z.gcd (env' "y") (env' "x" - env' "y")).
+        apply Z.gcd_comm.
+        rewrite H3.
+        assert (Z.gcd (env' "x") (env' "y") = Z.gcd (env' "y") (env' "x")).
+        apply Z.gcd_comm.
+        rewrite H4.
+        apply Z.gcd_sub_diag_r.
+    + intros.
+      split.
+      * lia.
+      * rewrite <-H1.
+        assert (env' "x" = env' "y").
+        lia.
+        rewrite H2.
+        apply Z.gcd_diag.
+Qed.
 
 Definition factorielle n :=
   Seq
@@ -128,7 +182,26 @@ Proof.
   intros.
   apply auto_hoare'; simpl.
   unfold update_state; simpl; intros.
-Admitted.
+  split.
+  - rewrite H0.
+    lia.
+  - intros.
+    split.
+    + intros.
+      rewrite <-H3.
+      symmetry.
+      rewrite Zfact_pos.
+      rewrite Z.mul_assoc.
+      reflexivity.
+      apply H2.
+    + intros.
+      assert (env' "n" <= 0).
+      lia.
+      apply Zfact_neg in H4.
+      rewrite H4 in H3.
+      rewrite Z.mul_1_r in H3.
+      apply H3.
+Qed.
 
 (* On définit la condition [a <= b] comme étant [a = b || a < b] *)
 Definition Le a b := Or (Eq a b) (Lt a b).
@@ -140,7 +213,7 @@ Example div_mod a b :=
       (Assign "y" (Const 0))
       (While
         (Le (Const b) (Var "x"))
-           (fun env => True)
+        (fun env =>  b * (env "y") + (env "x") = a)
         (Seq
           (Assign "x" (Sub (Var "x") (Const b)))
           (Assign "y" (Add (Var "y") (Const 1)))
@@ -154,7 +227,21 @@ Theorem div_mod_correct a b:
     (div_mod a b)
     (fun env => b * env "y" + env "x" = a /\ env "x" < b).
 Proof.
-Admitted.
+  intros.
+  apply auto_hoare'; simpl.
+  unfold update_state; simpl; intros.
+  split.
+  - lia.
+  - intros.
+    split.
+    + intros.
+      rewrite <- H2.
+      lia.
+    + intros.
+      split.
+      * apply H2.
+      * lia.
+Qed.
 
 Definition parity x :=
   Seq
@@ -163,7 +250,7 @@ Definition parity x :=
       (If (Lt (Const 0) (Var "x")) Skip (Assign "x" (Sub (Const 0) (Var "x"))))
       (While
         (Le (Const 2) (Var "x"))
-           (fun env => True)
+           (fun env => Z.even (env "x") = Z.even x /\ env "x" >= 0)
         (Assign "x" (Sub (Var "x") (Const 2)))
       )
     ).
@@ -183,7 +270,75 @@ Theorem parity_correct x:
        end
     ).
 Proof.
-Admitted.
+  intros.
+  apply auto_hoare'; simpl.
+  unfold update_state; simpl; intros.
+  split.
+  - intros.
+    split.
+    + split.
+      * reflexivity.
+      * lia.
+    + intros.
+      split.
+      * intros.
+        split.
+        -- destruct H3.
+           rewrite <-H3.
+           rewrite Z.even_sub. 
+           simpl.
+           destruct (Z.even (env' "x")).
+           tauto.
+           tauto.
+        -- destruct H2.
+           lia.
+           lia.
+      * intros.
+        destruct H3.
+        destruct (env' "x").
+        -- simpl in H3.
+           rewrite <-H3.
+           reflexivity.
+        -- destruct p.
+           ++ lia.
+           ++ lia.
+           ++ simpl in H3.
+              rewrite <-H3.
+              reflexivity.
+        -- lia.
+  - intros.
+    split.
+    + split.
+      * apply Z.even_opp.
+      * lia.
+    + intros.
+      split.
+      * intros.
+        destruct H3.
+        split.
+        -- rewrite <-H3.
+           rewrite Z.even_sub.
+           simpl.
+           destruct (Z.even (env' "x")).
+           tauto.
+           tauto.
+        -- destruct H2.
+           lia.
+           lia.
+      * intros.
+        destruct H3.
+        destruct (env' "x").
+        -- simpl in H3.
+           rewrite <-H3.
+           reflexivity.
+        -- destruct p.
+           ++ lia.
+           ++ lia.
+           ++ simpl in H3.
+              rewrite <-H3.
+              reflexivity.
+        -- lia.
+Qed.
 
 Definition sqrt x :=
   Seq
@@ -192,7 +347,7 @@ Definition sqrt x :=
       (Assign "z" (Const 0))
       (While
         (Le (Mul (Add (Var "z") (Const 1)) (Add (Var "z") (Const 1))) (Var "x"))
-           (fun env => True)
+           (fun env => env "z" * env "z" <= x)
         (Assign "z" ((Add (Var "z") (Const 1))))
       )
     ).
@@ -207,7 +362,31 @@ Theorem sqrt_correct x:
         /\ x < (env "z" + 1) * (env "z" + 1)
       ).
 Proof.
-Admitted.
+  intros.
+  apply auto_hoare'; simpl.
+  unfold update_state; simpl; intros.
+  split.
+  - lia.
+  - intros.
+    assert (env' "x" = x).
+    specialize (H1 "x").
+    simpl in H1.
+    symmetry.
+    apply H1.
+    intro.
+    destruct H2.
+    discriminate.
+    apply H2.
+    split.
+    + intros.
+      rewrite <-H2.
+      lia.
+    + intros.
+      rewrite <-H2.
+      split.
+      * lia.
+      * lia.
+Qed.
 
 Definition square1 x :=
   Seq
@@ -218,7 +397,7 @@ Definition square1 x :=
         (Assign "z" (Const 0))
         (While
           (Not (Eq (Var "y") (Const 0)))
-             (fun env => True)
+             (fun env => env "x" = x /\ env "z" = x * (x - env "y"))
           (Seq
             (Assign "z" (Add (Var "z") (Var "x")))
             (Assign "y" (Sub (Var "y") (Const 1)))
@@ -233,7 +412,25 @@ Theorem square1_correct x:
     (square1 x)
     (fun env => env "z" = x * x).
 Proof.
-Admitted.
+  intros.
+  apply auto_hoare'; simpl.
+  unfold update_state; simpl; intros.
+  split.
+  - split.
+    + reflexivity.
+    + lia.
+  - intros.
+    split.
+    + intros.
+      destruct H2.
+      split.
+      * apply H2.
+      * rewrite H3.
+        lia.
+    + intros.
+      destruct H2.
+      lia.
+Qed.
 
 Definition square2 x :=
   Seq
@@ -244,7 +441,7 @@ Definition square2 x :=
         (Assign "z" (Const 0))
         (While
           (Not (Eq (Var "y") (Var "x")))
-             (fun env => True)
+             (fun env => env "x" = x /\ env "z" + x * (env "x" - env "y") = x * x)
           (Seq
             (Assign "z" (Add (Var "z") (Var "x")))
             (Assign "y" (Add (Var "y") (Const 1)))
@@ -259,7 +456,21 @@ Theorem square2_correct x:
     (square2 x)
     (fun env => env "z" = x * x).
 Proof.
-Admitted.
+  intros.
+  apply auto_hoare'; simpl.
+  unfold update_state; simpl; intros.
+  split.
+  - lia.
+  - intros.
+    split.
+    + intros.
+      destruct H2.
+      split.
+      * apply H2.
+      * lia.
+    + intros.
+      lia.
+Qed.
 
 Check Zfib.
 
@@ -272,7 +483,7 @@ Definition Fib n :=
         (Assign "z" (Const 1))
         (While
           (Not (Eq (Var "x") (Const (1 + n))))
-          (fun env => True)
+          (fun env => 0 < env"x" /\ env "x" <= n + 1 /\ env "y" = Zfib (env "x" - 1) /\ env "z" = Zfib (env "x"))
           (Seq
             (Assign "t" (Var "z"))
             (Seq
@@ -296,5 +507,58 @@ Theorem fib_correct n:
   0 <= n
   -> valid_hoare_triple (fun env => True) (Fib n) (fun env => env "y" = Zfib n).
 Proof.
-Admitted.
+  intros.
+  apply auto_hoare'; simpl.
+  unfold update_state; simpl; intros.
+  split.
+  - split.
+    + lia.
+    + split.
+      * lia.
+      * split.
+        -- assert (1 - 1 = 0).
+           lia.
+           rewrite H1.
+           unfold Zfib.
+           simpl.
+           reflexivity.
+        -- unfold Zfib.
+           simpl.
+           reflexivity.
+  - intros.
+    split.
+    + intros.
+      destruct H3.
+      destruct H4.
+      destruct H5.
+      split.
+      * lia.
+      * split.
+        -- lia.
+        -- split.
+           ++ assert (env' "x" + 1 - 1 = env' "x").
+              lia.
+              rewrite H7.
+              rewrite H6.
+              reflexivity.
+            ++ rewrite H6.
+               rewrite H5.
+               assert (env' "x" + 1 = 1 + env' "x").
+               lia.
+               rewrite H7.
+               apply Zfib_eqn.
+               lia.
+    + intros.
+      destruct H3.
+      destruct H4.
+      destruct H5.
+      rewrite H5.
+      assert (env' "x" = n + 1).
+      lia.
+      rewrite H7.
+      assert (n + 1 - 1 = n).
+      lia.
+      rewrite H8.
+      reflexivity.
+Qed.
 
